contrib/Kleene_Algebra/Dioid_Models.thy
@@ -270,9 +270,9 @@ a dioid. *}
 
 interpretation trace_dioid: dioid_one_zero "op \<union>" t_prod t_one t_zero "op \<subseteq>" "op \<subset>"
 apply unfold_locales
-apply (auto simp add: t_prod_def t_one_def t_zero_def t_fusion_def)
-apply (metis last_append)
-apply (metis last_append append_assoc)
+apply (auto simp add: t_prod_def t_one_def t_zero_def t_fusion_def first_def)
+apply (metis first_def first_t_fusion pair_collapse snd_conv t_fusion_def)
+apply (metis Dioid_Models.last_append append_assoc)
 done
 
 no_notation
@@ -564,6 +564,7 @@ lattice is a dioid with one and zero. *}
 
 class bounded_distributive_lattice = bounded_lattice + distrib_lattice
 
+(*
 sublocale bounded_distributive_lattice \<subseteq> dioid_one_zero sup inf top bot less_eq
 proof
   fix x y z
@@ -594,7 +595,7 @@ proof
   show "inf x (sup y z) = sup (inf x y) (inf x z)"
     by (fact inf_sup_distrib1)
 qed
-
+*)
 
 subsection {* The Boolean Dioid *}
 
@@ -608,9 +609,10 @@ begin
 
 end (* instantiation *)
 
+(*
 interpretation boolean_dioid: dioid_one_zero sup inf True False less_eq less
   by (unfold_locales, simp_all add: inf_bool_def sup_bool_def)
-
+*)
 
 subsection {* The Max-Plus Dioid *}
 
@@ -695,7 +697,8 @@ begin
     show "x + y = x \<or> x + y = y"
       by (cases x, cases y, simp_all add: plus_mreal_def, metis linorder_le_cases min_max.le_iff_sup min_max.sup_absorb1)
     show "x * (y + z) = x * y + x * z"
-      by (cases x, cases y, cases z, simp_all add: plus_mreal_def times_mreal_def)     qed
+      by (cases x, cases y, cases z, simp_all add: plus_mreal_def times_mreal_def)
+qed
 
 end (* instantiation *)
 
