contrib/Kleene_Algebra/Omega_Algebra.thy
@@ -7,7 +7,7 @@
 header {* Omega Algebras *}
 
 theory Omega_Algebra
-imports Kleene_Algebra
+imports Kleene_Algebras
 begin
 
 text {*
@@ -48,6 +48,7 @@ lemma omega_coinduct_eq_var1: "y = 1 + x \<cdot> y \<longrightarrow> y \<le> x\<
 lemma  omega_coinduct_eq_var2: "y = x \<cdot> y \<longrightarrow> y \<le> x\<^sup>\<omega>"
   by (metis eq_refl omega_coinduct_var2)
 
+(*
 lemma "y = x \<cdot> y + z \<longrightarrow> y = x\<^sup>\<star> \<cdot> z + x\<^sup>\<omega>"
   nitpick [expect=genuine] -- "2-element counterexample"
 oops
@@ -59,6 +60,7 @@ oops
 lemma "y = x \<cdot> y \<longrightarrow> y = x\<^sup>\<omega>"
   nitpick [expect=genuine] -- "2-element counterexample"
 oops
+*)
 
 text {* Next we strengthen the unfold law to an equation. *}
 
@@ -75,9 +77,11 @@ qed
 lemma omega_unfold_var: "z + x \<cdot> x\<^sup>\<omega> \<le> x\<^sup>\<omega> + x\<^sup>\<star> \<cdot> z"
   by (metis add_lub add_ub1 omega_coinduct omega_unfold_eq)
 
+(*
 lemma "z + x \<cdot> x\<^sup>\<omega> = x\<^sup>\<omega> + x\<^sup>\<star> \<cdot> z"
   nitpick [expect=genuine] -- "4-element counterexample"
 oops
+*)
 
 text {* We now prove subdistributivity and isotonicity of omega. *}
 
@@ -141,9 +145,11 @@ proof -
     by (metis mult.assoc omega_coinduct_var2)
 qed
 
+(*
 lemma "x\<^sup>\<omega> \<cdot> y = x\<^sup>\<omega>"
   nitpick [expect=genuine] -- "2-element counterexample"
 oops
+*)
 
 lemma omega_sup_id: "1 \<le> y \<longrightarrow> x\<^sup>\<omega> \<cdot> y = x\<^sup>\<omega>"
   by (metis eq_iff mult_isol mult_oner omega_1)
@@ -154,9 +160,11 @@ lemma omega_top [simp]: "x\<^sup>\<omega> \<cdot> \<top> = x\<^sup>\<omega>"
 lemma supid_omega: "1 \<le> x \<longrightarrow> x\<^sup>\<omega> = \<top>"
   by (metis eq_iff max_element omega_iso top_def)
 
+(*
 lemma "x\<^sup>\<omega> = \<top> \<longrightarrow> 1 \<le> x"
   nitpick [expect=genuine] -- "4-element counterexample"
 oops
+*)
 
 text {* Next we prove a simulation law for the omega operation *}
 
@@ -171,6 +179,7 @@ proof
     by (metis calculation mult.assoc omega_coinduct_var2)
 qed
 
+(*
 lemma "z \<cdot> x \<le> y \<cdot> z \<longrightarrow> z \<cdot> x\<^sup>\<omega> \<le> y\<^sup>\<omega> \<cdot> z"
   nitpick -- "4-element counterexample"
 oops
@@ -182,6 +191,7 @@ oops
 lemma "y \<cdot> z  \<le> z \<cdot> x \<longrightarrow> y\<^sup>\<omega> \<cdot> z \<le> x\<^sup>\<omega>"
   nitpick -- "4-element counterexample"
 oops
+*)
 
 text {* Next we prove transitivity of omega elements. *}
 
@@ -285,7 +295,7 @@ text {* The next law shows how omegas below a sum can be unfolded. *}
 lemma omega_sum_unfold: "x\<^sup>\<omega> + x\<^sup>\<star> \<cdot> y \<cdot> (x + y)\<^sup>\<omega> = (x + y)\<^sup>\<omega>"
 proof -
   have "(x + y)\<^sup>\<omega> = x \<cdot> (x + y)\<^sup>\<omega> + y \<cdot> (x+y)\<^sup>\<omega>"
-    by (metis left_distrib omega_unfold_eq)
+    by (metis distrib_right omega_unfold_eq)
   thus ?thesis
     by (metis mult.assoc wagner_3)
 qed
@@ -374,12 +384,12 @@ lemma bachmair_dershowitz:
   shows "(x + y)\<^sup>\<omega> = 0 \<longleftrightarrow> x\<^sup>\<omega> + y\<^sup>\<omega> = 0"
 proof
   assume "(x + y)\<^sup>\<omega> = 0"
-  show "x\<^sup>\<omega> + y\<^sup>\<omega> = 0"
-    by (metis `(x + y)\<^sup>\<omega> = (0\<Colon>'a)` add.commute add_zero_r annir omega_sum_unfold)
+  thus "x\<^sup>\<omega> + y\<^sup>\<omega> = 0"
+    by (metis add.commute add_zero_r annir omega_sum_unfold)
 next
   assume "x\<^sup>\<omega> + y\<^sup>\<omega> = 0"
-  show "(x + y)\<^sup>\<omega> = 0"
-    by (metis `x\<^sup>\<omega> + y\<^sup>\<omega> = (0\<Colon>'a)` assms no_trivial_inverse omega_sum_refine right_distrib star_omega_1)
+  thus "(x + y)\<^sup>\<omega> = 0"
+    by (metis assms no_trivial_inverse omega_sum_refine distrib_left star_omega_1)
 qed
 
 text {*
@@ -394,9 +404,11 @@ where "ewp x \<equiv> \<not>(\<forall>y. y \<le> x \<cdot> y \<longrightarrow> y
 lemma ewp_super_id1: "0 \<noteq> 1 \<longrightarrow> 1 \<le> x \<longrightarrow> ewp x"
   by (metis ewp_def mult_oner)
 
+(*
 lemma "0 \<noteq> 1 \<longrightarrow> 1 \<le> x \<longleftrightarrow> ewp x"
   nitpick -- "3-element counterexample"
 oops
+*)
 
 text {* The next facts relate the absence of the empty word property
 with the absence of infinite iteration. *}
@@ -461,7 +473,7 @@ next
   also have "z + x \<cdot> y = z + x \<cdot> x\<^sup>\<star> \<cdot> z"
     by (metis calculation mult.assoc)
   moreover have "... = (1 + x \<cdot> x\<^sup>\<star>) \<cdot> z"
-    by (metis left_distrib mult_onel)
+    by (metis distrib_right mult_onel)
   moreover have "... = x\<^sup>\<star> \<cdot> z"
     by (metis star_unfoldl_eq)
   thus "z + x \<cdot> y = y"
