theories/core/utp_recursion.thy
@@ -10,7 +10,7 @@ theory utp_recursion
 imports 
   utp_lattice
   "../laws/utp_rel_laws"
-  "../algebra/Kleene_Algebra/Kleene_Algebra2"
+(*  "../algebra/Kleene_Algebra/Kleene_Algebras" *)
 begin
 
 subsection {* Fixed Points *}
@@ -187,77 +187,6 @@ done
 
 lemma UNREST_StarP [unrest]: "UNREST NON_REL_VAR p \<Longrightarrow> UNREST NON_REL_VAR (p\<^sup>\<star>)"
   by (auto intro:unrest simp add:star_WF_PREDICATE_def)
-
-interpretation rel_dioid: dioid_one_zero "op \<union>" "op O" Id "{}" "op \<subseteq>" "op \<subset>"
-  by (unfold_locales, auto)
-
-interpretation rel_monoid: monoid_mult Id "op O" ..
-
-lemma power_is_relpow: "rel_dioid.power X n = X ^^ n"
-proof (induct n)
-  case 0 show ?case
-    by (metis rel_dioid.power_0 relpow.simps(1))
-  case Suc thus ?case
-    by (metis rel_dioid.power_Suc2 relpow.simps(2))
-qed
-
-lemma rel_star_def: "X^* = (\<Union>n. rel_dioid.power X n)"
-  by (simp add: power_is_relpow rtrancl_is_UN_relpow)
-
-lemma rel_star_contl: "X O Y^* = (\<Union>n. X O rel_dioid.power Y n)"
-by (metis rel_star_def relcomp_UNION_distrib)
-
-lemma rel_star_contr: "X^* O Y = (\<Union>n. (rel_dioid.power X n) O Y)"
-by (metis rel_star_def relcomp_UNION_distrib2)
-
-context dioid_one_zero
-begin
-
-lemma power_inductl: "z + x \<cdot> y \<le> y \<longrightarrow> (x ^ n) \<cdot> z \<le> y"
-proof (induct n)
-  case 0 show ?case
-    by (metis add_lub mult_onel power_0)
-  case Suc thus ?case
-    by (auto, metis add_lub mult.assoc mult_isol order_trans)
-qed
-
-lemma power_inductr: "z + y \<cdot> x \<le> y \<longrightarrow> z \<cdot> (x ^ n) \<le> y"
-proof (induct n)
-  case 0 show ?case
-    by (metis add_lub mult_oner power_0)
-  case Suc
-  {
-    fix n
-    assume "z + y \<cdot> x \<le> y \<longrightarrow> z \<cdot> x ^ n \<le> y"
-      and "z + y \<cdot> x \<le> y"
-    hence "z \<cdot> x ^ n \<le> y"
-      by auto
-    also have "z \<cdot> x ^ Suc n = z \<cdot> x \<cdot> x ^ n"
-      by (metis mult.assoc power_Suc)
-    moreover have "... = (z \<cdot> x ^ n) \<cdot> x"
-      by (metis mult.assoc power_commutes)
-    moreover have "... \<le> y \<cdot> x"
-      by (metis calculation(1) mult_isor)
-    moreover have "... \<le> y"
-      by (metis `z + y \<cdot> x \<le> y` add_lub)
-    ultimately have "z \<cdot> x ^ Suc n \<le> y" by auto
-  }
-  thus ?case
-    by (metis Suc)
-qed
-
-end (* dioid_one_zero *)
-
-interpretation rel_kleene_algebra: kleene_algebra "op \<union>" "op O" Id "{}" "op \<subseteq>" "op \<subset>" rtrancl
-proof
-  fix x y z :: "'a rel"
-  show "Id \<union> x O x\<^sup>* \<subseteq> x\<^sup>*"
-    by (metis order_refl r_comp_rtrancl_eq rtrancl_unfold)
-  show "z \<union> x O y \<subseteq> y \<longrightarrow> x\<^sup>* O z \<subseteq> y"
-    by (simp only: rel_star_contr, metis (lifting) SUP_le_iff rel_dioid.power_inductl)
-  show "z \<union> y O x \<subseteq> y \<longrightarrow> z O x\<^sup>* \<subseteq> y"
-    by (simp only: rel_star_contl, metis (lifting) SUP_le_iff rel_dioid.power_inductr)
-qed
 
 instantiation WF_PREDICATE :: (VALUE) dioid
 begin
